
\[
  \begin{prooftree}
    \Hypo{ \vdash \implies \varphi, \psi }
    \Infer1{ \vdash \psi \land \varphi }
  \end{prooftree}
\]

$\psi \implies \varphi$\
$\underline{\chi \implies \varphi \quad\quad\quad\quad\quad\quad\quad\quad\quad\quad\quad}$\
$((\psi \land \varphi) \iff (\chi \land \varphi)) \iff (\psi \iff \chi)$


$\underline{\psi \land \varphi}$\
$\psi$

$\psi \implies \varphi$\
$\underline{\psi\quad\quad}$\
$\psi \land \varphi$

$\psi \land \varphi \vdash \psi$\
$\underline{\psi \implies \varphi, \psi \vdash \psi \land \varphi}$\
$\psi \iff (\psi \land \varphi)$


$\underline{\chi \land \varphi}$\
$\chi$

$\chi \implies \varphi$\
$\underline{\chi\quad\quad\quad}$\
$\chi \land \varphi$

$\chi \land \varphi \vdash \chi$\
$\underline{\chi \implies \varphi, \chi \vdash \chi \land \varphi}$\
$\chi \iff (\chi \land \varphi)$


$\psi \iff (\psi \land \varphi)$\
$\chi \iff (\chi \land \varphi)$\
$\underline{(\psi \land \varphi) \implies (\chi \land \varphi)}$\
$\psi \implies \chi$


$\underline{\psi \land \varphi}$\
$\varphi \land \psi$

$\underline{\chi \land \varphi}$\
$\chi \land \psi$

$\psi \iff (\psi \land \varphi)$\
$\chi \iff (\chi \land \varphi)$\
$\underline{(\chi \land \varphi) \implies (\psi \land \varphi)}$\
$\chi \implies \psi$


$\psi \implies \chi$\
$\underline{\chi \implies \psi}$\
$\psi \iff \chi$